src/Parsers/DependentlyTypedMinimalOfParseFactoredFull.v
@@ -1,0 +1,94 @@
+(** * Definition of a [comp]-based non-computational CFG parser *)
+Require Import Coq.Lists.List Coq.Program.Program Coq.Program.Wf Coq.Arith.Wf_nat Coq.Arith.Compare_dec Coq.Classes.RelationClasses Coq.Strings.String.
+Require Import Parsers.ContextFreeGrammar Parsers.Specification Parsers.DependentlyTyped Parsers.MinimalParse.
+Require Parsers.BooleanRecognizer Parsers.BooleanRecognizerCorrect.
+Require Import Parsers.DependentlyTypedMinimalOfParseFactored.
+Require Import Parsers.WellFoundedParse Parsers.ContextFreeGrammarProperties.
+Require Import Common Common.ilist Common.Wf Common.Le.
+
+Set Implicit Arguments.
+
+Local Open Scope string_like_scope.
+
+Local Coercion is_true : bool >-> Sortclass.
+
+Section recursive_descent_parser.
+  Context (G : grammar Ascii.ascii).
+
+  Local Instance predata : parser_computational_predataT
+    := { nonterminal_names_listT := BooleanRecognizer.rdp_list_names_listT;
+         initial_nonterminal_names_data := Valid_nonterminal_symbols G;
+         is_valid_nonterminal_name := BooleanRecognizer.rdp_list_is_valid_name;
+         remove_nonterminal_name := BooleanRecognizer.rdp_list_remove_name;
+         nonterminal_names_listT_R := BooleanRecognizer.rdp_list_names_listT_R;
+         remove_nonterminal_name_dec := BooleanRecognizer.rdp_list_remove_name_dec;
+         ntl_wf := BooleanRecognizer.rdp_list_ntl_wf }.
+
+  Local Instance types_data : @parser_computational_types_dataT _ string_stringlike
+    := {| predata := predata;
+          split_stateT str0 valid g str := True |}.
+
+  Local Instance methods' : @parser_computational_dataT' _ string_stringlike types_data
+    := { split_string_for_production str0 valid it its := BooleanRecognizer.make_all_single_splits;
+         split_string_for_production_correct str0 valid it its str
+         := Forall_impl _ _ (BooleanRecognizer.make_all_single_splits_correct_eq str)
+}.
+  Proof.
+    intros; apply bool_eq_correct; assumption.
+  Defined.
+
+  Local Instance strdata : @parser_computational_prestrdataT _ string_stringlike G {| DependentlyTyped.methods' := methods' |} idM.
+  Proof.
+    constructor; simpl; intros; assumption.
+  Defined.
+
+  Local Instance orig_methods : @parser_computational_dataT _ string_stringlike
+    := { methods' := methods' }.
+
+  Lemma rdp_list_complete'
+        (str0 : string_stringlike) (valid : nonterminal_names_listT)
+        (it : item Ascii.ascii) (its : production Ascii.ascii)
+        (str : StringWithSplitState string_stringlike (split_stateT str0 valid (it :: its : production _)))
+        (pf : str ≤s str0)
+  : DependentlyTypedMinimal.split_list_completeT G valid it its str pf
+                                                 (split_string_for_production str0 valid it its str).
+  Proof.
+    simpl.
+    repeat intro.
+    apply (@BooleanRecognizerCorrect.make_all_single_splits_complete
+             G BooleanRecognizer.rdp_list_names_listT
+             (Valid_nonterminal_symbols G)
+             BooleanRecognizer.rdp_list_is_valid_name
+             BooleanRecognizer.rdp_list_remove_name
+             {| string_val := str0 : string_stringlike ; state_val := I |}
+             valid valid
+             str
+             pf (it::its : production _)).
+    assumption.
+  Defined.
+
+  Global Instance minimal_of_parse_parser_dependent_types_extra_data
+  : @parser_dependent_types_extra_dataT _ string_stringlike G
+    := @minimal_of_parse_parser_dependent_types_extra_data'
+         _ string_stringlike G
+         predata methods' strdata
+         BooleanRecognizer.rdp_list_remove_name_1 BooleanRecognizer.rdp_list_remove_name_2
+         rdp_list_complete'.
+
+  Definition minimal_parse_nonterminal_name__of__parse
+             (nonterminal_name : string)
+             (s : string)
+             (p : parse_of_item string_stringlike G s (NonTerminal _ nonterminal_name))
+             (H : Forall_parse_of_item
+                    (fun _ n => is_valid_nonterminal_name initial_nonterminal_names_data n = true)
+                    p)
+  : minimal_parse_of_name string_stringlike G initial_nonterminal_names_data is_valid_nonterminal_name remove_nonterminal_name s initial_nonterminal_names_data s nonterminal_name.
+  Proof.
+    eapply @minimal_parse_nonterminal_name__of__parse'.
+    exact strdata.
+    exact BooleanRecognizer.rdp_list_remove_name_1.
+    exact BooleanRecognizer.rdp_list_remove_name_2.
+    exact rdp_list_complete'.
+    exact H.
+  Defined.
+End recursive_descent_parser.
